commit

Projects/Esolangs/Lang_001/Basic.lean
@@ -1,5 +1,7 @@
 import Projects.Esolangs.Lang_001.Defs
 
+attribute [-simp] List.getElem!_eq_getElem?_getD
+
 namespace Esolangs.Lang_001
 
 def exprId : Expr :=
@@ -26,6 +28,29 @@ def exprZero : Expr :=
 def exprOne : Expr :=
   call (.builtin .succ) [refZero]
 
+def exprNot : Expr :=
+  call (.builtin .sub) [refOne, .arg 0]
+
+def exprBool : Expr :=
+  call (.custom 3) [call (.custom 3) [.arg 0]]
+
+def exprAdd : Expr :=
+  call (.builtin .sub)
+    [ call (.builtin .sub)
+      [ call (.builtin .sub)
+        [ call (.builtin .succ) [call (.builtin .succ) [
+            call (.custom 5)
+              [ call (.builtin .sub) [.arg 0, refOne]
+              , call (.builtin .sub) [.arg 1, refOne]
+              ]
+          ]]
+        , call (.custom 3) [.arg 0]
+        ]
+      , call (.custom 3) [.arg 1]
+      ]
+    , call (.custom 5) [refZero, refZero]
+    ]
+
 def exprMain₁ : Expr :=
   exprId
 
@@ -34,6 +59,18 @@ def prog₁ : Prog where
     ⟨1, exprMain₁⟩,
     ⟨0, exprZero⟩,
     ⟨0, exprOne⟩,
+    ⟨1, exprNot⟩,
+    ⟨1, exprBool⟩,
+    -- ⟨2, exprAdd⟩,
+  ]
+
+def prog₁FS : List (List ℕ → ℕ) :=
+  [ fn 1 λ xs => xs[0]!
+  , fn 0 λ _ => 0
+  , fn 0 λ _ => 1
+  , fn 1 λ xs => if xs[0]! = 0 then 1 else 0
+  , fn 1 λ xs => if xs[0]! = 0 then 0 else 1
+  -- , fn 2 λ xs => xs[0]! + xs[1]!
   ]
 
 -- #check 0 #exit
@@ -46,7 +83,7 @@ def prog₁ : Prog where
 @[simp] theorem wf_defId : (Def.mk 1 (.arg 0)).WF progId := wf_exprId
 @[simp] theorem arity_zero_progId : progId.arity 0 = 1 := rfl
 @[simp] theorem expr_zero_progId : progId.expr 0 = exprId := rfl
-@[simp] theorem Expr.eval_arg {i prog f args} : (arg i).eval prog f args = args[i]! := rfl
+@[simp] theorem Expr.run_arg {i prog f args} : (arg i).eval prog f args = args[i]! := rfl
 @[simp] theorem Prog.defs_mk {ds} : defs ⟨ds⟩ = ds := rfl
 @[simp] theorem Builtin.arity_succ : Builtin.succ.arity = 1 := rfl
 @[simp] theorem Builtin.arity_sub : Builtin.sub.arity = 2 := rfl
@@ -55,6 +92,7 @@ def prog₁ : Prog where
 @[simp] theorem Target.f_custom {fs i} : (custom i).f fs = fs[i]! := rfl
 @[simp] theorem Target.arity_custom {prog i} : (custom i).arity prog = prog.arity i := rfl
 @[simp] theorem Prog.main_mk {defs} : main ⟨defs⟩ = defs[0]! := rfl
+@[simp] theorem Expr.wf_arg {prog n i} : (arg i).WF prog n ↔ i < n := by rfl
 
 @[simp, instance]
 theorem wf_progId : progId.WF := by
@@ -66,11 +104,11 @@ theorem wf_progId : progId.WF := by
   obtain ⟨f, rfl⟩ := h₁; simp at h₂ h₃ ⊢; grind
 
 @[simp]
-theorem Expr.eval_call' {prog fs args t xs} : (Expr.call' t xs).eval prog fs args =
+theorem Expr.run_call' {prog fs args t xs} : (Expr.call' t xs).eval prog fs args =
 t.f fs (List.range (t.arity prog) |>.map λ i => xs i |>.eval prog fs args) := rfl
 
 @[simp]
-theorem Expr.eval_call {prog fs args t xs} : (call t xs).eval prog fs args =
+theorem Expr.run_call {prog fs args t xs} : (call t xs).eval prog fs args =
 t.f fs (List.range (t.arity prog) |>.map λ i => xs[i]! |>.eval prog fs args) := rfl
 
 theorem not_wf_progSelf : ¬progSelf.WF := by
@@ -86,13 +124,13 @@ theorem Prog.compatible_fs {prog : Prog} [H : prog.WF] : prog.Compatible prog.fs
   Classical.epsilon_spec # H.exiu_compatible.exists
 
 @[simp]
-theorem eval_progId {n} : progId.eval n = n := by
-  simp [Prog.eval, Prog.eval']; have h := @progId.compatible_fs.eval_eq
+theorem run_progId {n} : progId.run n = n := by
+  simp [Prog.run, Prog.eval]; have h := @progId.compatible_fs.eval_eq
   simp at h; specialize @h [n]; simp at h; exact h
 
 @[simp]
 theorem wf_expr_prog₁_main₁ : exprMain₁.WF prog₁ 1 := by
-  constructor; simp
+  constructor
 
 @[simp]
 theorem wf_def_prog₁_main₁ : Def.WF prog₁ ⟨1, exprMain₁⟩ := by
@@ -110,124 +148,126 @@ prog.HasTarget (.custom i) ↔ i < prog.defs.length := by rfl
 @[simp] theorem Builtin.f_succ : f .succ = (·[0]! + 1) := rfl
 @[simp] theorem Builtin.f_sub : f .sub = (λ xs => xs[0]! - xs[1]!) := rfl
 
------
-
-@[simp] theorem length_defs_prog₁ : prog₁.defs.length = 3 := rfl
+@[simp]
+theorem Expr.wf_call' {prog t args n} : (call' t args).WF prog n ↔ prog.HasTarget t ∧
+∀ ⦃j⦄, if t.arity prog ≤ j then args j = default else args j |>.WF prog n := by rfl
 
 @[simp]
-theorem wf_prog₁_refZero : refZero.WF prog₁ 0 := by
-  constructor <;> simp [prog₁]
+theorem Expr.wf_call {prog t args n} : (call t args).WF prog n ↔ prog.HasTarget t ∧
+∀ ⦃j⦄, if t.arity prog ≤ j then args[j]! = default else args[j]! |>.WF prog n := by rfl
 
-@[simp]
-theorem wf_prog₁_refOne : refOne.WF prog₁ 0 := by
-  constructor <;> simp [prog₁]
+theorem Prog.fs_eq_of_compatible {prog : Prog} {fs} [hp : prog.WF]
+(h : prog.Compatible fs) : prog.fs = fs :=
+  hp.exiu_compatible.unique prog.compatible_fs h
 
-@[simp]
-theorem wf_expr_prog₁_exprZero : exprZero.WF prog₁ 0 := by
-  constructor <;> simp; intro i; split_ifs with h; grind; simp at h
-  rw [show [_, _] = .replicate 2 _ by rfl]
-  rw [List.getElem?_eq_getElem h, List.getElem_replicate]; simp
+instance {prog : Prog} {i} : Decidable # prog.HasDef i := by
+  unfold Prog.HasDef; infer_instance
 
-@[simp]
-theorem wf_expr_prog₁_exprOne : exprOne.WF prog₁ 0 := by
-  constructor <;> simp; intro i; split_ifs with h; grind; simp at h; simp [h]
-
-@[simp]
-theorem wf_def_prog₁_exprZero : Def.WF prog₁ ⟨0, exprZero⟩ := by
-  simp [Def.WF]
-
-@[simp]
-theorem wf_def_prog₁_exprOne : Def.WF prog₁ ⟨0, exprOne⟩ := by
-  simp [Def.WF]
+instance {prog : Prog} {t} : Decidable # prog.HasTarget t := by
+  unfold Prog.HasTarget; cases t <;> infer_instance
 
 -- #check 0 #exit
 
-@[simp] theorem arity_prog₁_0 : prog₁.arity 0 = 1 := rfl
-@[simp] theorem arity_prog₁_1 : prog₁.arity 1 = 0 := rfl
-@[simp] theorem arity_prog₁_2 : prog₁.arity 2 = 0 := rfl
+-----
+
+@[simp] theorem length_defs_prog₁ : prog₁.defs.length = 5 := rfl
+
+@[simp] theorem prog₁_arity_0 : prog₁.arity 0 = 1:= rfl
+@[simp] theorem prog₁_arity_1 : prog₁.arity 1 = 0:= rfl
+@[simp] theorem prog₁_arity_2 : prog₁.arity 2 = 0:= rfl
+@[simp] theorem prog₁_arity_3 : prog₁.arity 3 = 1:= rfl
+@[simp] theorem prog₁_arity_4 : prog₁.arity 4 = 1:= rfl
+-- @[simp] theorem prog₁_arity_5 : prog₁.arity 5 = 2:= rfl
+
+@[simp]
+theorem wf_prog₁_refZero {n} : refZero.WF prog₁ n := by
+  constructor <;> simp [prog₁]
+
+@[simp]
+theorem wf_expr_prog₁_exprZero {n} : exprZero.WF prog₁ n := by
+  constructor <;> simp; intro i; split_ifs with h; grind; simp at h
+  rw [show [_, _] = .replicate 2 _ by rfl]
+  rw [List.getElem!_eq_getElem h, List.getElem_replicate]; simp
+
+@[simp]
+theorem wf_prog₁_refOne {n} : refOne.WF prog₁ n := by
+  constructor <;> simp [prog₁]
+
+@[simp]
+theorem wf_expr_prog₁_exprOne {n} : exprOne.WF prog₁ n := by
+  constructor <;> simp; intro i; split_ifs with h; grind; simp at h; simp [h]
+
+@[simp]
+theorem wf_expr_prog₁_exprNot {n} : exprNot.WF prog₁ n ↔ 1 ≤ n := by
+  simp [exprNot]; constructor; contrapose!; simp; rintro rfl; use 1; simp
+  intro h i; split_ifs with h₁; grind
+  obtain rfl | rfl : i = 0 ∨ i = 1 := by omega
+  all_goals simp <;> omega
+
+@[simp]
+theorem wf_expr_prog₁_exprBool {n} : exprBool.WF prog₁ n ↔ 1 ≤ n := by
+  simp [exprBool]; constructor
+  · contrapose!; simp; rintro rfl; use 0; simp; use 0; simp
+  · intro h i; split_ifs with h₁; grind; simp at h₁; simp [h₁]
+    intro j; split_ifs with h₂; grind; simp at h₂; simp [h₂]; omega
+
+-- #check 0 #exit
+
+@[simp]
+theorem compatible_prog₁_prog₁FS : prog₁.Compatible prog₁FS := by
+  unfold prog₁FS; constructor <;> simp
+  all_goals
+    intro i h xs h₁
+    obtain rfl | rfl | rfl | rfl | rfl :
+      i = 0 ∨ i = 1 ∨ i = 2 ∨ i = 3 ∨ i = 4 := by omega
+  iterate 6 simp at h₁; simp [fn] <;> try grind
+  all_goals nth_rw 1 [prog₁]; (try simp at h₁); simp [fn, h₁]
+  · simp [exprMain₁, exprId]
+  · simp [exprZero]
+  · simp [exprOne, refZero, fn]
+  · simp [exprNot, refOne, fn]; grind
+  · simp [exprBool, fn]; grind
+  -- · simp [exprAdd, fn]; rw! [xs.eq_getElem_of_length_eq_two h₁]
+  --   simp; generalize xs[0] = x; generalize xs[1] = y; clear h₁ xs
+  --   simp [refOne, refZero, fn]; cases x; cases y <;> rfl; nm x
+  --   simp; cases y; rfl; nm y; simp; omega
+
+-- #check 0 #exit
 
 @[simp, instance]
 theorem wf_prog₁ : prog₁.WF := by
-  constructor
-  · rintro ⟨⟩
-  · rfl
-  · nth_rw 1 [prog₁]; simp
-  use [fn 1 (·[0]!), fn 0 λ _ => 0, fn 0 λ _ => 1]
-  simp
-  constructor
-  · constructor <;> simp
-    · intro i h xs h₁
-      replace h : i = 0 ∨ i = 1 ∨ i = 2; omega
-      rcases h with rfl | rfl | rfl <;> simp at h₁ <;> simp [fn] <;> grind
-    · rintro i h xs h₁
-      replace h : i = 0 ∨ i = 1 ∨ i = 2; omega
-      nth_rw 1 [prog₁]
-      rcases h with rfl | rfl | rfl <;> simp at h₁ <;> simp [fn]
-      · simp [exprMain₁, exprId, h₁]
-      · simp [exprZero]
-      · simp [exprOne, h₁, refZero, fn]
-  rintro fs ⟨h₁, h₂, h₃⟩
-  simp at h₁ h₂ h₃
-  rw [List.ext_getElem_iff]
-  simp [h₁]
-  intro i h₄ h₅
-  have h_zero : fs[1] [] = 0
+  constructor; rintro ⟨⟩; rfl; nth_rw 1 [prog₁]; simp
+  use prog₁FS, (by simp); unfold prog₁FS
+  rintro fs ⟨h₁, h₂, h₃⟩; simp at h₁ h₂ h₃
+  have h_zero : fs[1]! [] = 0
   · specialize @h₃ 1 (by omega) [] (by simp)
-    simp [prog₁, exprZero] at h₃
-    rw [List.getElem?_eq_getElem # by grind] at h₃
-    simp at h₃
-    exact h₃
-  specialize h₂ h₄
-  specialize h₃ h₄
-  ext xs
-  specialize @h₂ xs
-  specialize @h₃ xs
-  have h₆ : i = 0 ∨ i = 1 ∨ i = 2; omega
-  rcases h₆ with rfl | rfl | rfl
-  · simp [fn] at h₂ h₃ ⊢
-    split_ifs with H
-    · clear h₂
-      specialize h₃ H
-      simp [prog₁, exprMain₁, exprId] at h₃
-      rw [List.length_eq_one_iff] at H
-      obtain ⟨x, rfl⟩ := H
-      simp at h₃ ⊢
-      rw [List.getElem?_eq_getElem # by grind] at h₃
-      simp at h₃
-      exact h₃
-    · clear h₃
-      specialize h₂ H
-      rw [List.getElem?_eq_getElem # by grind] at h₂
-      simp at h₂
-      exact h₂
-  · simp [fn, prog₁, exprZero] at h₂ h₃ ⊢
-    rw [List.getElem?_eq_getElem # by grind] at h₂ h₃
-    simp at h₂ h₃
-    nth_rw 2 [eq_comm] at h₃
-    tauto
-  · simp [fn, prog₁] at h₂ h₃ ⊢
-    rw [List.getElem?_eq_getElem # by grind] at h₂ h₃
-    simp at h₂ h₃
-    simp [exprOne, refZero] at h₃
-    rw [List.getElem?_eq_getElem # by grind] at h₃
-    simp at h₃
-    split_ifs with H
-    rotate_left; exact h₂ H
-    clear h₂
-    subst H
-    specialize h₃ rfl
-    rw [h₃]; clear h₃
-    simpa
+    simp [prog₁, exprZero] at h₃; exact h₃
+  have h_one : fs[2]! [] = 1
+  · specialize @h₃ 2 (by omega) [] (by simp)
+    simp [prog₁, exprOne, refZero] at h₃; grind
+  have h_not : ∀ ⦃x⦄, fs[3]! [x] = if x = 0 then 1 else 0
+  · intro x; specialize @h₃ 3 (by omega) [x] (by simp)
+    simp [prog₁, exprNot, refOne] at h₃; grind
+  rw [List.ext_getElem!_iff]; simp [h₁]; intro i h₄; ext xs
+  specialize @h₂ i (by omega); specialize @h₃ i (by omega)
+  specialize @h₂ xs; specialize @h₃ xs
+  obtain rfl | rfl | rfl | rfl | rfl :
+    i = 0 ∨ i = 1 ∨ i = 2 ∨ i = 3 ∨ i = 4 := by omega
+  all_goals simp [prog₁, fn] at h₂ h₃ ⊢
+  · split_ifs with H
+    · specialize h₃ H; simp [exprMain₁, exprId] at h₃; grind
+    · specialize h₂ H; grind
+  · simp [exprZero] at h₃; grind
+  · simp [exprOne] at h₂ h₃; grind
+  · simp [exprNot, refOne] at h₂ h₃; grind
+  · simp [exprBool] at h₂ h₃; grind
+
+-- #check 0 #exit
 
 @[simp]
-theorem prog₁_eval'_zero : prog₁.eval' 1 [] = 0 := by
-  simp [Prog.eval']; have h := @prog₁.compatible_fs.eval_eq; simp at h
-  specialize @h 1 (by omega) [] rfl
-  rw [h]; simp [prog₁, exprZero]
+theorem fs_prog₁ : prog₁.fs = prog₁FS :=
+  Prog.fs_eq_of_compatible compatible_prog₁_prog₁FS
 
 @[simp]
-theorem prog₁_eval'_one : prog₁.eval' 2 [] = 1 := by
-  simp [Prog.eval']; have h := @prog₁.compatible_fs.eval_eq; simp at h
-  specialize @h 2 (by omega) [] rfl; rw [h]; clear h
-  nth_rw 1 [prog₁]; simp [exprOne, refZero]
-  convert prog₁_eval'_zero; ext; simp [Prog.eval']
+theorem run_prog₁ {x} : prog₁.run x = x := by
+  simp [Prog.run, Prog.eval, prog₁FS, fn]
